Specs for several more functions and their litmus tests (with first, non-ergonomic proofs)

rocq-brick-libstdcpp/test/cstring/test.cpp
@@ -130,8 +130,153 @@ void test_search_embedded_null_array_buffer() {
     assert(std::strstr(s, "") == s);
 }
 
+void test_memchr() {
+    unsigned char s[] = {'a', 'b', 'c', 'a'};
+    assert(std::memchr(s, 'a', 4) == s);
+    assert(std::memchr(s, 'c', 4) == s + 2);
+    assert(std::memchr(s, 'z', 4) == nullptr);
+    assert(std::memchr(s, 'a', 0) == nullptr);
+    assert(std::memchr(s + 1, 'a', 3) == s + 3);
+}
+
+void test_memchr_embedded_null() {
+    unsigned char s[] = {'a', '\0', 'b', '\0'};
+    assert(std::memchr(s, '\0', 4) == s + 1);
+    assert(std::memchr(s + 2, '\0', 2) == s + 3);
+    assert(std::memchr(s, 'b', 4) == s + 2);
+}
+
+void test_memcmp() {
+    unsigned char abc[] = {'a', 'b', 'c'};
+    unsigned char abd[] = {'a', 'b', 'd'};
+    unsigned char ab[] = {'a', 'b'};
+
+    assert(std::memcmp(abc, abc, 3) == 0);
+    assert(std::memcmp(abc, abd, 3) < 0);
+    assert(std::memcmp(abd, abc, 3) > 0);
+    assert(std::memcmp(abc, abd, 2) == 0);
+    assert(std::memcmp(abc, ab, 0) == 0);
+}
+
+void test_memcmp_embedded_null() {
+    unsigned char x[] = {'a', '\0', 'x'};
+    unsigned char y[] = {'a', '\0', 'y'};
+
+    assert(std::memcmp(x, y, 2) == 0);
+    assert(std::memcmp(x, y, 3) < 0);
+    assert(std::memcmp(y, x, 3) > 0);
+}
+
+void test_memset() {
+    unsigned char s[] = {'a', 'b', 'c', 'd'};
+
+    assert(std::memset(s, 'x', 2) == s);
+    assert(s[0] == 'x');
+    assert(s[1] == 'x');
+    assert(s[2] == 'c');
+    assert(s[3] == 'd');
+
+    assert(std::memset(s + 2, 0x123, 1) == s + 2);
+    assert(s[2] == static_cast<unsigned char>(0x123));
+    assert(s[3] == 'd');
+}
+
+void test_memset_embedded_null() {
+    unsigned char s[] = {'a', 'b', 'c', 'd'};
+
+    assert(std::memset(s + 1, '\0', 2) == s + 1);
+    assert(s[0] == 'a');
+    assert(s[1] == '\0');
+    assert(s[2] == '\0');
+    assert(s[3] == 'd');
+}
+
+void test_memcpy() {
+    unsigned char src[] = {'a', 'b', 'c', 'd'};
+    unsigned char dst[] = {'w', 'x', 'y', 'z'};
+
+    assert(std::memcpy(dst, src, 3) == dst);
+    assert(dst[0] == 'a');
+    assert(dst[1] == 'b');
+    assert(dst[2] == 'c');
+    assert(dst[3] == 'z');
+    assert(src[0] == 'a');
+    assert(src[3] == 'd');
+
+    assert(std::memcpy(dst + 1, src + 2, 0) == dst + 1);
+    assert(dst[0] == 'a');
+    assert(dst[1] == 'b');
+}
+
+void test_memcpy_embedded_null() {
+    unsigned char src[] = {'a', '\0', 'b', '\0'};
+    unsigned char dst[] = {'w', 'x', 'y', 'z'};
+
+    assert(std::memcpy(dst, src, 4) == dst);
+    assert(dst[0] == 'a');
+    assert(dst[1] == '\0');
+    assert(dst[2] == 'b');
+    assert(dst[3] == '\0');
+}
+
+void test_memmove() {
+    unsigned char src[] = {'a', 'b', 'c', 'd'};
+    unsigned char dst[] = {'w', 'x', 'y', 'z'};
+
+    assert(std::memmove(dst, src, 4) == dst);
+    assert(dst[0] == 'a');
+    assert(dst[1] == 'b');
+    assert(dst[2] == 'c');
+    assert(dst[3] == 'd');
+
+    assert(std::memmove(dst + 1, src + 1, 0) == dst + 1);
+    assert(dst[1] == 'b');
+}
+
+void test_memmove_overlap() {
+    char forward[] = {'a', 'b', 'c', 'd', 'e', 'f', '\0'};
+    char backward[] = {'a', 'b', 'c', 'd', 'e', 'f', '\0'};
+
+    assert(std::memmove(forward + 2, forward, 4) == forward + 2);
+    assert(forward[0] == 'a');
+    assert(forward[1] == 'b');
+    assert(forward[2] == 'a');
+    assert(forward[3] == 'b');
+    assert(forward[4] == 'c');
+    assert(forward[5] == 'd');
+    assert(forward[6] == '\0');
+
+    assert(std::memmove(backward, backward + 2, 4) == backward);
+    assert(backward[0] == 'c');
+    assert(backward[1] == 'd');
+    assert(backward[2] == 'e');
+    assert(backward[3] == 'f');
+    assert(backward[4] == 'e');
+    assert(backward[5] == 'f');
+    assert(backward[6] == '\0');
+}
+
+void test_memmove_embedded_null() {
+    char s[] = {'a', '\0', 'b', 'c', '\0'};
+
+    assert(std::memmove(s + 1, s, 4) == s + 1);
+    assert(s[0] == 'a');
+    assert(s[1] == 'a');
+    assert(s[2] == '\0');
+    assert(s[3] == 'b');
+    assert(s[4] == 'c');
+}
+
 void test_cstring_slice1() {
     test_strlen();
     test_strcmp();
     test_strncmp();
+}
+
+void test_cstring_slice4() {
+    test_memchr();
+    test_memcmp();
+    test_memset();
+    test_memcpy();
+    test_memmove();
 }
