rocq-brick-libstdcpp/test/cstring/proof.v
@@ -5,9 +5,21 @@
  *)
 Require Import skylabs.auto.cpp.proof.
 Require Import skylabs.auto.cpp.hints.anyR.
+(** BEGIN: SKYLABS DEFAULT PROOF IMPORTS *)
+Require Import skylabs.auto.cpp.prelude.proof.
+Require Import skylabs.cpp.array.
+Import expr_join.
+#[local] Hint Resolve delayed_case.smash_delayed_case_B | 1000 : br_hints.
+#[local] Hint Resolve delayed_case.expr_join.smash_delayed_case_B | 1000 : br_hints.
+(** END: SKYLABS DEFAULT PROOF IMPORTS *)
 Require Import skylabs.brick.libstdcpp.cassert.spec.
 Require Import skylabs.brick.libstdcpp.cstring.spec.
 Require Import skylabs.brick.libstdcpp.test.cstring.test_cpp.
+
+Import normalize.only_provable_norm.
+
+Import normalize.normalize_ptr.
+Import refine_lib.
 
 #[local] Lemma borrow_arrayR_cstringR `{Σ : cpp_logic, σ : genv}
     (p : ptr) q bytes s tail :
@@ -32,11 +44,81 @@ Proof.
     iFrame.
 Qed.
 
+#[local] Lemma borrow_arrayLR_cstringR `{Σ : cpp_logic, σ : genv}
+    (p : ptr) q bytes s tail :
+  bytes = cstring.to_zstring s ++ tail ->
+  cstring.WF s ->
+  p |-> arrayLR (Tchar_ char_type.Cchar) 0 (lengthZ bytes)
+          (fun c : N => charR q c) bytes ⊢
+  p |-> cstring.R q s ∗
+  (p |-> cstring.R q s -∗
+   p |-> arrayLR (Tchar_ char_type.Cchar) 0 (lengthZ bytes)
+           (fun c : N => charR q c) bytes).
+Proof.
+  intros Hbytes Hwf.
+  rewrite arrayLR.unlock _at_sep.
+  iIntros "[_ Harr]".
+  rewrite _at_offsetR _at_sub_0; [|done].
+  iPoseProof (borrow_arrayR_cstringR p q bytes s tail Hbytes Hwf with "Harr")
+    as "[Hs Hclose]".
+  iSplitL "Hs".
+  - iExact "Hs".
+  - iIntros "Hs".
+    iPoseProof ("Hclose" with "Hs") as "Harr".
+    rewrite /arrayLR.
+    iSplit.
+    + iPureIntro. lia.
+    + iExact "Harr".
+Qed.
+
 #[local] Lemma offset_entails `{Σ : cpp_logic, σ : genv}
     (o : offset) (P Q : Rep) :
   (P ⊢ Q) -> o |-> P ⊢ o |-> Q.
 Proof.
   intros HPQ. apply _offsetR_mono. exact HPQ.
+Qed.
+
+#[local] Lemma at_zero_intro `{Σ : cpp_logic, σ : genv}
+    (p : ptr) (R : Rep) :
+  p |-> R ⊢ p .[Tuchar ! 0] |-> R.
+Proof.
+  rewrite _at_sub_0; [reflexivity|done].
+Qed.
+
+#[local] Lemma at_zero_elim `{Σ : cpp_logic, σ : genv}
+    (p : ptr) (R : Rep) :
+  p .[Tuchar ! 0] |-> R ⊢ p |-> R.
+Proof.
+  rewrite _at_sub_0; [reflexivity|done].
+Qed.
+
+#[local] Lemma at_type_ptrR_validR_plus_one `{Σ : cpp_logic, σ : genv}
+    (p : ptr) ty :
+  p |-> type_ptrR ty ⊢ p .[ty ! 1] |-> validR.
+Proof.
+  rewrite -_at_offsetR.
+  apply heap_pred._at_cancel.
+  apply type_ptrR_validR_plus_one.
+Qed.
+
+#[local] Lemma at_uchar_offset_add_intro `{Σ : cpp_logic, σ : genv}
+    (p : ptr) i j k (R : Rep) :
+  k = (i + j)%Z ->
+  p .[Tuchar ! k] |-> R ⊢ p .[Tuchar ! i] .[Tuchar ! j] |-> R.
+Proof.
+  intros ->.
+  rewrite o_sub_sub.
+  reflexivity.
+Qed.
+
+#[local] Lemma at_uchar_offset_add_elim `{Σ : cpp_logic, σ : genv}
+    (p : ptr) i j k (R : Rep) :
+  k = (i + j)%Z ->
+  p .[Tuchar ! i] .[Tuchar ! j] |-> R ⊢ p .[Tuchar ! k] |-> R.
+Proof.
+  intros ->.
+  rewrite o_sub_sub.
+  reflexivity.
 Qed.
 
 #[local] Lemma arrayR_charR_Vchar `{Σ : cpp_logic, σ : genv} q xs :
@@ -75,8 +157,379 @@ Proof.
   exact Hlen.
 Qed.
 
+#[local] Lemma arrayLR_charR_anyR `{Σ : cpp_logic, σ : genv} (p : ptr) n xs :
+  N.to_nat n = length xs ->
+  p |-> arrayLR (Tchar_ char_type.Cchar) 0 (Z.of_N n)
+         (fun c : N => charR 1$m c) xs ⊢
+  p |-> anyR (Tarray (Tchar_ char_type.Cchar) n) 1$m.
+Proof.
+  intros Hlen.
+  rewrite arrayLR.unlock _at_sep.
+  iIntros "[_ Harr]".
+  rewrite _at_offsetR _at_sub_0; [|done].
+  iApply (arrayR_charR_anyR with "Harr").
+  exact Hlen.
+Qed.
+
+#[local] Lemma at_charR_anyR `{Σ : cpp_logic, σ : genv}
+    (p : ptr) q x :
+  p |-> charR q x ⊢ p |-> anyR (Tchar_ char_type.Cchar) q.
+Proof.
+  apply heap_pred._at_cancel.
+  apply primR_anyR.
+Qed.
+
+#[local] Lemma arrayR_charR_arrayR_anyR `{Σ : cpp_logic, σ : genv}
+    (p : ptr) xs :
+  p |-> arrayR (Tchar_ char_type.Cchar) (fun c : N => charR 1$m c) xs ⊢
+  p |-> arrayR (Tchar_ char_type.Cchar)
+         (fun _ : unit => anyR (Tchar_ char_type.Cchar) 1$m)
+         (replicateN (lengthN xs) ()).
+Proof.
+  revert p.
+  induction xs as [|x xs IH].
+  all: intros p.
+  - rewrite /lengthN /= !arrayR_nil. reflexivity.
+  - rewrite arrayR_cons !_at_sep _at_offsetR.
+    iIntros "(Hty & Hx & Hxs)".
+    replace (lengthN (x :: xs)) with (N.succ (lengthN xs)) by
+      (rewrite /lengthN Nat2N.inj_succ; reflexivity).
+    rewrite replicateN_S.
+    rewrite arrayR_cons !_at_sep _at_offsetR.
+    iFrame "Hty".
+    iSplitL "Hx".
+    + iApply (at_charR_anyR with "Hx").
+    + iApply (IH with "Hxs").
+Qed.
+
+#[local] Lemma arrayLR_charR_arrayLR_anyR `{Σ : cpp_logic, σ : genv}
+    (p : ptr) n xs :
+  N.to_nat n = length xs ->
+  p |-> arrayLR (Tchar_ char_type.Cchar) 0 (Z.of_N n)
+         (fun c : N => charR 1$m c) xs ⊢
+  p |-> arrayLR (Tchar_ char_type.Cchar) 0 (Z.of_N n)
+         (fun _ : unit => anyR (Tchar_ char_type.Cchar) 1$m)
+         (replicateN n ()).
+Proof.
+  intros Hlen.
+  rewrite arrayLR.unlock _at_sep.
+  iIntros "[_ Harr]".
+  rewrite _at_offsetR _at_sub_0; [|done].
+  replace (replicateN n ()) with (replicateN (lengthN xs) ())
+    by (rewrite /replicateN /lengthN -(N2Nat.id n) Hlen; reflexivity).
+  iPoseProof (arrayR_charR_arrayR_anyR with "Harr") as "Harr".
+  rewrite /arrayLR.
+  iSplit.
+  - iPureIntro.
+    unfold lengthZ, lengthN, replicateN.
+    rewrite length_replicate.
+    replace (length xs) with (N.to_nat n) by exact Hlen.
+    repeat rewrite N2Nat.id.
+    lia.
+  - rewrite _at_offsetR _at_sub_0; [|done].
+    iExact "Harr".
+Qed.
+
+#[local] Lemma arrayLR_prefix_tail0 `{Σ : cpp_logic, σ : genv}
+    {A : Type} (p : ptr) ty mid hi (R : A -> Rep) xs0 xs1 :
+  lengthN xs0 = Z.to_N mid ->
+  (0 <= mid)%Z ->
+  (mid <= hi)%Z ->
+  p |-> arrayLR ty 0 hi R (xs0 ++ xs1) ⊣⊢
+  p |-> arrayLR ty 0 mid R xs0 ∗
+  p .[ty ! mid] |-> arrayLR ty 0 (hi - mid) R xs1.
+Proof.
+  intros Hlen Hlo Hhi.
+  assert (Hlen' : lengthN xs0 = Z.to_N (mid - 0)) by
+    (replace (mid - 0)%Z with mid by lia; exact Hlen).
+  rewrite (arrayLR_app' p 0 mid hi R xs0 xs1 Hlen' Hlo Hhi).
+  rewrite _at_sub_arrayLR.
+  Arith.arith_simpl.
+  reflexivity.
+Qed.
+
+#[local] Lemma arrayR_ucharR_object_bytesR `{Σ : cpp_logic, σ : genv}
+    (p : ptr) xs :
+  p |-> arrayR Tuchar (fun b : Z => ucharR 1$m b) xs ⊢
+  p |-> object_bytesR Tuchar 1$m xs.
+Proof.
+  iIntros "Hs".
+  iApply object_bytesR_of_arrayLR; [reflexivity|].
+  rewrite arrayLR.unlock _at_sep.
+  iSplit; [iPureIntro; lia|].
+  rewrite _at_offsetR _at_sub_0; [iExact "Hs"|done].
+Qed.
+
+#[local] Lemma object_bytesR_half_split `{Σ : cpp_logic, σ : genv}
+    (p : ptr) ty bytes :
+  p |-> object_bytesR ty 1$m bytes ⊣⊢
+  p |-> object_bytesR ty (cQp.mk false (1/2)) bytes ∗
+  p |-> object_bytesR ty (cQp.mk false (1/2)) bytes.
+Proof.
+  rewrite -(cfractional (P := fun q => p |-> object_bytesR ty q bytes)
+    (cQp.mk false (1/2)) (cQp.mk false (1/2))).
+  rewrite -cQp.mk_add' Qp.half_half.
+  reflexivity.
+Qed.
+
+#[local] Lemma object_bytesR_prefix_tail0 `{Σ : cpp_logic, σ : genv}
+    (p : ptr) ty q mid hi xs0 xs1 :
+  lengthZ (xs0 ++ xs1) = hi ->
+  lengthZ xs0 = mid ->
+  lengthZ xs1 = (hi - mid)%Z ->
+  p |-> object_bytesR ty q (xs0 ++ xs1) ⊣⊢
+  p |-> object_bytesR ty q xs0 ∗
+  p .[ty ! mid] |-> object_bytesR ty q xs1.
+Proof.
+  intros Htotal Hhead Htail.
+  iSplit.
+  - iIntros "Hs".
+    iPoseProof (object_bytesR_to_arrayLR p ty q hi (xs0 ++ xs1)
+      Htotal with "Hs") as "Hs".
+    iPoseProof (arrayLR_prefix_tail0 p ty mid hi
+      (fun b : Z => ucharR q b) xs0 xs1
+      ltac:(rewrite <- Hhead; rewrite N2Z.id; reflexivity)
+      ltac:(lia) ltac:(lia) with "Hs") as "[Hhead Htail]".
+    iPoseProof (object_bytesR_of_arrayLR p ty q mid xs0
+      Hhead with "Hhead") as "Hhead".
+    iPoseProof (object_bytesR_of_arrayLR (p .[ ty ! mid]) ty q
+      (hi - mid) xs1 Htail with "Htail") as "Htail".
+    iFrame.
+  - iIntros "[Hhead Htail]".
+    iPoseProof (object_bytesR_to_arrayLR p ty q mid xs0
+      Hhead with "Hhead") as "Hhead".
+    iPoseProof (object_bytesR_to_arrayLR (p .[ ty ! mid]) ty q
+      (hi - mid) xs1 Htail with "Htail") as "Htail".
+    iPoseProof ((arrayLR_prefix_tail0 p ty mid hi
+      (fun b : Z => ucharR q b) xs0 xs1
+      ltac:(rewrite <- Hhead; rewrite N2Z.id; reflexivity)
+      ltac:(lia) ltac:(lia)) with "[$Hhead $Htail]") as "Hs".
+    iPoseProof (object_bytesR_of_arrayLR p ty q hi
+      (xs0 ++ xs1) Htotal with "Hs") as "Hs".
+    iExact "Hs".
+Qed.
+
+#[local] Lemma arrayLR_ucharR_anyR `{Σ : cpp_logic, σ : genv} (p : ptr) n xs :
+  N.to_nat n = length xs ->
+  p |-> arrayLR Tuchar 0 (Z.of_N n) (fun c : Z => ucharR 1$m c) xs ⊢
+  p |-> anyR (Tarray Tuchar n) 1$m.
+Proof.
+  intros Hlen.
+  rewrite arrayLR.unlock _at_sep.
+  iIntros "[_ Harr]".
+  rewrite _at_offsetR _at_sub_0; [|done].
+  rewrite anyR_array.
+  iApply (arrayR_anyR_f (fun c : Z => c) with "Harr").
+  exact Hlen.
+Qed.
+
+#[local] Lemma lengthZ_of_to_nat_length {A : Type} (n : N) (xs : list A) :
+  N.to_nat n = length xs -> lengthZ xs = Z.of_N n.
+Proof.
+  intros Hlen.
+  unfold lengthZ, lengthN.
+  rewrite <- Hlen, N2Nat.id.
+  reflexivity.
+Qed.
+
+#[local] Lemma memchr_found_after_prefix prefix b suffix c :
+  List.Forall (fun x => x <> byte_of_int c) prefix ->
+  b = byte_of_int c ->
+  memchr (prefix ++ b :: suffix) c = Some (Z.of_nat (length prefix)).
+Proof.
+  intros Hprefix Hb.
+  induction Hprefix as [|x prefix Hx _ IH].
+  - simpl.
+    rewrite bool_decide_true; [|done].
+    reflexivity.
+  - simpl.
+    rewrite bool_decide_false; [|done].
+    rewrite IH.
+    simpl.
+    f_equal.
+    rewrite Nat2Z.inj_succ.
+    rewrite Z.add_1_l.
+    reflexivity.
+Qed.
+
+#[local] Lemma memchr_missing_if_no_match bytes c :
+  List.Forall (fun x => x <> byte_of_int c) bytes ->
+  memchr bytes c = None.
+Proof.
+  intros Hbytes.
+  induction Hbytes as [|x bytes Hx _ IH].
+  - reflexivity.
+  - simpl.
+    rewrite bool_decide_false; [|done].
+    rewrite IH.
+    reflexivity.
+Qed.
+
+#[local] Ltac solve_memchr_side :=
+  unfold byte_of_int;
+  repeat (rewrite Z.mod_small; [|lia]);
+  match goal with
+  | |- List.Forall _ [] => constructor
+  | |- List.Forall _ (_ :: _) =>
+      constructor; [solve_memchr_side | solve_memchr_side]
+  | |- _ => lia
+  end.
+
+#[local] Lemma object_bytesR_ucharR_anyR `{Σ : cpp_logic, σ : genv}
+    (p : ptr) n xs :
+  N.to_nat n = length xs ->
+  p |-> object_bytesR Tuchar 1$m xs ⊢
+  p |-> anyR (Tarray Tuchar n) 1$m.
+Proof.
+  intros Hlen.
+  iIntros "Hs".
+  iPoseProof (object_bytesR_to_arrayLR p Tuchar 1$m (Z.of_N n) xs
+    ltac:(apply lengthZ_of_to_nat_length; exact Hlen)
+    with "Hs") as "Hs".
+  iApply (arrayLR_ucharR_anyR with "Hs").
+  exact Hlen.
+Qed.
+
+#[local] Lemma object_bytesR_ucharR_object_bytes_anyR
+    `{Σ : cpp_logic, σ : genv} (p : ptr) n xs :
+  N.to_nat n = length xs ->
+  p |-> object_bytesR Tuchar 1$m xs ⊢
+  p |-> object_bytes_anyR Tuchar (Z.of_N n).
+Proof.
+  intros Hlen.
+  iIntros "Hs".
+  iPoseProof (object_bytesR_ucharR_anyR _ n xs Hlen with "Hs") as "Hs".
+  iApply (object_bytes_anyR_of_anyR_array with "Hs").
+Qed.
+
+#[local] Lemma object_bytesR_ucharR_arrayR `{Σ : cpp_logic, σ : genv}
+    (p : ptr) xs :
+  p |-> object_bytesR Tuchar 1$m xs ⊢
+  p |-> arrayR Tuchar (fun b : Z => ucharR 1$m b) xs.
+Proof.
+  iIntros "Hs".
+  iPoseProof (object_bytesR_to_arrayLR p Tuchar 1$m (lengthZ xs) xs
+    eq_refl with "Hs") as "Hs".
+  rewrite arrayLR.unlock _at_sep.
+  iDestruct "Hs" as "[_ Hs]".
+  rewrite _at_offsetR _at_sub_0; [iExact "Hs"|done].
+Qed.
+
+#[local] Lemma at_arrayR_ucharR_cons `{Σ : cpp_logic, σ : genv}
+    (p : ptr) x xs :
+  p |-> arrayR Tuchar (fun b : Z => ucharR 1$m b) (x :: xs) ⊣⊢
+  p |-> type_ptrR Tuchar ∗
+  p |-> ucharR 1$m x ∗
+  p .[Tuchar ! 1] |-> arrayR Tuchar (fun b : Z => ucharR 1$m b) xs.
+Proof.
+  rewrite arrayR_cons !_at_sep.
+  rewrite _at_offsetR.
+  reflexivity.
+Qed.
+
+#[local] Lemma at_arrayR_cons `{Σ : cpp_logic, σ : genv}
+    {A : Type} (p : ptr) ty (R : A -> Rep) x xs :
+  p |-> arrayR ty R (x :: xs) ⊣⊢
+  p |-> type_ptrR ty ∗
+  p |-> R x ∗
+  p .[ty ! 1] |-> arrayR ty R xs.
+Proof.
+  rewrite arrayR_cons !_at_sep.
+  rewrite _at_offsetR.
+  reflexivity.
+Qed.
+
+#[local] Lemma at_ucharR_anyR `{Σ : cpp_logic, σ : genv}
+    (p : ptr) q x :
+  p |-> ucharR q x ⊢ p |-> anyR Tuchar q.
+Proof.
+  apply heap_pred._at_cancel.
+  apply primR_anyR.
+Qed.
+
+#[local] Lemma arrayR_ucharR_arrayR_anyR `{Σ : cpp_logic, σ : genv}
+    (p : ptr) xs :
+  p |-> arrayR Tuchar (fun b : Z => ucharR 1$m b) xs ⊢
+  p |-> arrayR Tuchar (fun _ : unit => anyR Tuchar 1$m)
+    (replicateN (lengthN xs) ()).
+Proof.
+  revert p.
+  induction xs as [|x xs IH].
+  all: intros p.
+  - rewrite /lengthN /= !arrayR_nil. reflexivity.
+  - rewrite (at_arrayR_ucharR_cons p x xs).
+    iIntros "(Hty & Hx & Hxs)".
+    replace (lengthN (x :: xs)) with (N.succ (lengthN xs)) by
+      (rewrite /lengthN Nat2N.inj_succ; reflexivity).
+    rewrite replicateN_S.
+    rewrite (at_arrayR_cons p Tuchar
+      (fun _ : unit => anyR Tuchar 1$m) () (replicateN (lengthN xs) ())).
+    iFrame "Hty".
+    iSplitL "Hx".
+    + iApply (at_ucharR_anyR with "Hx").
+    + iApply (IH with "Hxs").
+Qed.
+
+#[local] Lemma object_bytesR_ucharR_arrayLR_anyR
+    `{Σ : cpp_logic, σ : genv} (p : ptr) n xs :
+  N.to_nat n = length xs ->
+  p |-> object_bytesR Tuchar 1$m xs ⊢
+  p |-> arrayLR Tuchar 0 (Z.of_N n)
+    (fun _ : unit => anyR Tuchar 1$m) (replicateN n ()).
+Proof.
+  intros Hlen.
+  iIntros "Hs".
+  iPoseProof (object_bytesR_ucharR_arrayR with "Hs") as "Hs".
+  rewrite arrayLR.unlock _at_sep.
+  iSplit.
+  - iPureIntro.
+    unfold lengthZ, lengthN, replicateN.
+    rewrite length_replicate N2Nat.id.
+    lia.
+  - 
+  rewrite _at_offsetR _at_sub_0; [|done].
+  rewrite -(N2Nat.id n) Hlen.
+  iApply (arrayR_ucharR_arrayR_anyR with "Hs").
+Qed.
+
+#[local] Lemma uchar_cells_object_bytesR_two `{Σ : cpp_logic, σ : genv}
+    (p : ptr) a b :
+  p |-> ucharR 1$m a ∗
+  p .[Tuchar ! 1] |-> ucharR 1$m b ⊢
+  p |-> object_bytesR Tuchar 1$m [a; b].
+Proof.
+  iIntros "(Ha & Hb)".
+  iDestruct (observe (p |-> type_ptrR Tuchar) with "Ha") as "#Hty0".
+  iDestruct (observe (p .[Tuchar ! 1] |-> type_ptrR Tuchar) with "Hb")
+    as "#Hty1".
+  iApply arrayR_ucharR_object_bytesR.
+  rewrite (at_arrayR_ucharR_cons p a [b]).
+  iFrame "Hty0 Ha".
+  rewrite (at_arrayR_ucharR_cons (p .[Tuchar ! 1]) b []).
+  iFrame "Hty1 Hb".
+  rewrite arrayR_nil _at_sep.
+  iSplit.
+  - iApply (at_type_ptrR_validR_plus_one with "Hty1").
+  - iPureIntro. done.
+Qed.
+
+#[local] Lemma arrayR_ucharR_anyR `{Σ : cpp_logic, σ : genv} (p : ptr) n xs :
+  N.to_nat n = length xs ->
+  p |-> arrayR Tuchar (fun b : Z => ucharR 1$m b) xs ⊢
+  p |-> anyR (Tarray Tuchar n) 1$m.
+Proof.
+  intros Hlen.
+  iIntros "Hs".
+  iPoseProof (arrayR_ucharR_object_bytesR with "Hs") as "Hs".
+  iApply (object_bytesR_ucharR_anyR with "Hs").
+  exact Hlen.
+Qed.
+
 Section with_cpp.
   Context `{Σ : cpp_logic} `{MOD : module ⊧ σ}.
+
+  (* Restored after the byte-array slice landed. This note records why these
+     proofs were parked temporarily during focused iteration. *)
 
   cpp.spec "test_strlen()" default.
   Lemma test_strlen_ok : verify[module] "test_strlen()".
@@ -110,7 +563,7 @@ Section with_cpp.
     verify[module] "test_strlen_array_buffer()".
   Proof.
     verify_spec; go.
-    iPoseProof (borrow_arrayR_cstringR _ _
+    iPoseProof (borrow_arrayLR_cstringR _ _
       (cstring.to_zstring "ab"%bs ++ [99%N; 100%N; 0%N]) "ab"%bs
       [99%N; 100%N; 0%N] eq_refl
       ltac:(apply cstring.WF_cons;
@@ -123,7 +576,7 @@ Section with_cpp.
     iSplit; [go|].
     iIntros "Hs".
     iPoseProof ("Hclose" with "Hs") as "Harr".
-    iPoseProof (arrayR_charR_anyR _ 6%N
+    iPoseProof (arrayLR_charR_arrayLR_anyR _ 6%N
       (cstring.to_zstring "ab"%bs ++ [99%N; 100%N; 0%N])
       ltac:(rewrite cstring.to_zstring_unfold; reflexivity) with "Harr")
       as "Harr".
@@ -137,7 +590,7 @@ Section with_cpp.
     verify[module] "test_strcmp_array_buffer()".
   Proof.
     verify_spec; go.
-    iPoseProof (borrow_arrayR_cstringR _ _
+    iPoseProof (borrow_arrayLR_cstringR _ _
       (cstring.to_zstring "ab"%bs ++ [120%N; 0%N]) "ab"%bs
       [120%N; 0%N] eq_refl
       ltac:(apply cstring.WF_cons;
@@ -146,7 +599,7 @@ Section with_cpp.
         [change (Byte.x62 <> Byte.x00); congruence|];
         apply cstring.WF_nil) with "[$]")
       as "[Hx Hclosex]".
-    iPoseProof (borrow_arrayR_cstringR _ _
+    iPoseProof (borrow_arrayLR_cstringR _ _
       (cstring.to_zstring "ab"%bs ++ [121%N; 0%N]) "ab"%bs
       [121%N; 0%N] eq_refl
       ltac:(apply cstring.WF_cons;
@@ -159,11 +612,11 @@ Section with_cpp.
     iIntros "[Hx Hy]".
     iPoseProof ("Hclosex" with "Hx") as "Harrx".
     iPoseProof ("Hclosey" with "Hy") as "Harry".
-    iPoseProof (arrayR_charR_anyR _ 5%N
+    iPoseProof (arrayLR_charR_arrayLR_anyR _ 5%N
       (cstring.to_zstring "ab"%bs ++ [120%N; 0%N])
       ltac:(rewrite cstring.to_zstring_unfold; reflexivity) with "Harrx")
       as "Harrx".
-    iPoseProof (arrayR_charR_anyR _ 5%N
+    iPoseProof (arrayLR_charR_arrayLR_anyR _ 5%N
       (cstring.to_zstring "ab"%bs ++ [121%N; 0%N])
       ltac:(rewrite cstring.to_zstring_unfold; reflexivity) with "Harry")
       as "Harry".
@@ -177,7 +630,7 @@ Section with_cpp.
     verify[module] "test_strncmp_array_buffer()".
   Proof.
     verify_spec; go.
-    iPoseProof (borrow_arrayR_cstringR _ _
+    iPoseProof (borrow_arrayLR_cstringR _ _
       (cstring.to_zstring "ab"%bs ++ [120%N; 0%N]) "ab"%bs
       [120%N; 0%N] eq_refl
       ltac:(apply cstring.WF_cons;
@@ -186,7 +639,7 @@ Section with_cpp.
         [change (Byte.x62 <> Byte.x00); congruence|];
         apply cstring.WF_nil) with "[$]")
       as "[Hx Hclosex]".
-    iPoseProof (borrow_arrayR_cstringR _ _
+    iPoseProof (borrow_arrayLR_cstringR _ _
       (cstring.to_zstring "ab"%bs ++ [121%N; 0%N]) "ab"%bs
       [121%N; 0%N] eq_refl
       ltac:(apply cstring.WF_cons;
@@ -199,11 +652,11 @@ Section with_cpp.
     iIntros "[Hx Hy]".
     iPoseProof ("Hclosex" with "Hx") as "Harrx".
     iPoseProof ("Hclosey" with "Hy") as "Harry".
-    iPoseProof (arrayR_charR_anyR _ 5%N
+    iPoseProof (arrayLR_charR_arrayLR_anyR _ 5%N
       (cstring.to_zstring "ab"%bs ++ [120%N; 0%N])
       ltac:(rewrite cstring.to_zstring_unfold; reflexivity) with "Harrx")
       as "Harrx".
-    iPoseProof (arrayR_charR_anyR _ 5%N
+    iPoseProof (arrayLR_charR_arrayLR_anyR _ 5%N
       (cstring.to_zstring "ab"%bs ++ [121%N; 0%N])
       ltac:(rewrite cstring.to_zstring_unfold; reflexivity) with "Harry")
       as "Harry".
@@ -256,7 +709,7 @@ Section with_cpp.
     verify[module] "test_search_embedded_null_array_buffer()".
   Proof using MOD.
     verify_spec; go.
-    iPoseProof (borrow_arrayR_cstringR _ _
+    iPoseProof (borrow_arrayLR_cstringR _ _
       (cstring.to_zstring "ab"%bs ++ [98%N; 99%N; 0%N]) "ab"%bs
       [98%N; 99%N; 0%N] eq_refl
       ltac:(apply cstring.WF_cons;
@@ -311,7 +764,7 @@ Section with_cpp.
     iIntros "[Hs Hempty]".
     Arith.arith_simpl; go; ego.
     iPoseProof ("Hclose" with "Hs") as "Harr".
-    iPoseProof (arrayR_charR_anyR _ 6%N
+    iPoseProof (arrayLR_charR_arrayLR_anyR _ 6%N
       (cstring.to_zstring "ab"%bs ++ [98%N; 99%N; 0%N])
       ltac:(rewrite cstring.to_zstring_unfold; reflexivity) with "Harr")
       as "Harr".
@@ -323,4 +776,773 @@ Section with_cpp.
   cpp.spec "test_cstring_slice1()" default.
   Lemma test_cstring_slice1_ok : verify[module] "test_cstring_slice1()".
   Proof. verify_spec; go. Qed.
+
+  cpp.spec "test_memset()" default.
+  Lemma test_memset_ok : verify[module] "test_memset()".
+  Proof using MOD _Σ thread_info Σ σ.
+    verify_spec; go.
+    iDestruct select (s_addr |-> arrayLR Tuchar 0 4
+      (fun v : Z => ucharR 1$m v) [97%Z; 98%Z; 99%Z; 100%Z]) as "Hs".
+    iPoseProof (object_bytesR_of_arrayLR s_addr Tuchar (cQp.mk false 1)
+      4 [97%Z; 98%Z; 99%Z; 100%Z] ltac:(reflexivity) with "Hs") as "Hs".
+
+    iPoseProof (object_bytesR_prefix_tail0 s_addr Tuchar
+      (cQp.mk false 1) 2 4 [97%Z; 98%Z] [99%Z; 100%Z]
+      ltac:(reflexivity) ltac:(reflexivity) ltac:(reflexivity) with "Hs")
+      as "[Htarget Htail]".
+    iExists Tuchar.
+    iSplitL "Htarget".
+    - iApply (object_bytesR_ucharR_object_bytes_anyR _ 2%N
+        [97%Z; 98%Z] ltac:(reflexivity) with "Htarget").
+    - iIntros "Htarget".
+      go.
+      iPoseProof ((object_bytesR_prefix_tail0 s_addr Tuchar
+        (cQp.mk false 1) 2 4 [120%Z; 120%Z] [99%Z; 100%Z]
+        ltac:(reflexivity) ltac:(reflexivity) ltac:(reflexivity))
+        with "[$Htarget $Htail]") as "Hs".
+      iPoseProof (object_bytesR_ucharR_arrayR with "Hs") as "Hs".
+      rewrite (at_arrayR_ucharR_cons s_addr 120%Z
+        [120%Z; 99%Z; 100%Z]).
+      iDestruct "Hs" as "[#Hty0 [H0 Hs]]".
+      iPoseProof (at_zero_intro s_addr with "H0") as "H0".
+      iExists (Vint 120%Z), (cQp.mk false 1%Qp).
+      iFrame "H0". iIntros "H0".
+      go.
+      iPoseProof (at_arrayR_ucharR_cons (s_addr .[Tuchar ! 1])
+        120%Z [99%Z; 100%Z] with "Hs") as "Hs".
+      iDestruct "Hs" as "[#Hty1 [H1 Hs]]".
+      iExists (Vint 120%Z), (cQp.mk false 1%Qp).
+      iFrame "H1". iIntros "H1".
+      go.
+      iPoseProof (at_arrayR_ucharR_cons
+        (s_addr .[Tuchar ! 1] .[Tuchar ! 1])
+        99%Z [100%Z] with "Hs") as "Hs".
+      iDestruct "Hs" as "[#Hty2 [H2 Hs]]".
+      iEval (rewrite o_sub_sub) in "H2".
+      iEval (rewrite o_sub_sub) in "Hs".
+      Arith.arith_simpl.
+      iExists (Vint 99%Z), (cQp.mk false 1%Qp).
+      iFrame "H2". iIntros "H2".
+      go.
+      iPoseProof (at_arrayR_ucharR_cons
+        (s_addr .[Tuchar ! 1] .[Tuchar ! 2])
+        100%Z [] with "Hs") as "Hs".
+      iDestruct "Hs" as "[#Hty3 [H3 Hs]]".
+      iEval (rewrite o_sub_sub) in "H3".
+      iEval (rewrite o_sub_sub) in "Hs".
+      Arith.arith_simpl.
+      iExists (Vint 100%Z), (cQp.mk false 1%Qp).
+      iFrame "H3". iIntros "H3".
+      go.
+      iPoseProof (at_zero_elim s_addr with "H0") as "H0".
+      iPoseProof (uchar_cells_object_bytesR_two s_addr 120%Z 120%Z
+        with "[$H0 $H1]") as "Hhead".
+      Arith.arith_simpl.
+      iPoseProof (at_uchar_offset_add_intro s_addr 2 1 3
+        (ucharR 1$m 100%Z) ltac:(lia) with "H3") as "H3".
+      iPoseProof (uchar_cells_object_bytesR_two (s_addr .[Tuchar ! 2])
+        99%Z 100%Z with "[$H2 $H3]") as "Htail".
+      iPoseProof (object_bytesR_prefix_tail0 (s_addr .[ Tuchar ! 2])
+        Tuchar (cQp.mk false 1) 1 2 [99%Z] [100%Z]
+        ltac:(reflexivity) ltac:(reflexivity) ltac:(reflexivity) with "Htail")
+        as "[Htarget Htail]".
+      iRename "Hs" into "Hempty".
+      go.
+      go.
+      iExists Tuchar.
+      iSplitL "Htarget".
+      + iApply (object_bytesR_ucharR_object_bytes_anyR _ 1%N
+          [99%Z] ltac:(reflexivity) with "Htarget").
+      + iIntros "Htarget".
+        go.
+        iPoseProof ((object_bytesR_prefix_tail0 (s_addr .[ Tuchar ! 2])
+          Tuchar (cQp.mk false 1) 1 2 [35%Z] [100%Z]
+          ltac:(reflexivity) ltac:(reflexivity) ltac:(reflexivity))
+          with "[$Htarget $Htail]") as "Htail".
+        iPoseProof ((object_bytesR_prefix_tail0 s_addr Tuchar
+          (cQp.mk false 1) 2 4 [120%Z; 120%Z] [35%Z; 100%Z]
+          ltac:(reflexivity) ltac:(reflexivity) ltac:(reflexivity))
+          with "[$Hhead $Htail]") as "Hs".
+        iPoseProof (object_bytesR_ucharR_arrayR with "Hs") as "Hs".
+        go.
+        rewrite (at_arrayR_ucharR_cons s_addr 120%Z
+          [120%Z; 35%Z; 100%Z]).
+        iDestruct "Hs" as "[#Hty0' [H0 Hs]]".
+        iPoseProof (at_zero_intro s_addr with "H0") as "H0_assert".
+        iPoseProof (at_arrayR_ucharR_cons (s_addr .[Tuchar ! 1])
+          120%Z [35%Z; 100%Z] with "Hs") as "Hs".
+        iDestruct "Hs" as "[#Hty1' [H1 Hs]]".
+        iPoseProof (at_arrayR_ucharR_cons
+          (s_addr .[Tuchar ! 1] .[Tuchar ! 1])
+          35%Z [100%Z] with "Hs") as "Hs".
+        iDestruct "Hs" as "[#Hty2' [H2 Hs]]".
+        iEval (rewrite o_sub_sub) in "H2".
+        iEval (rewrite o_sub_sub) in "Hs".
+        Arith.arith_simpl.
+        iExists (Vint 35%Z), (cQp.mk false 1%Qp).
+        iFrame "H2". iIntros "H2".
+        go.
+        iPoseProof (at_arrayR_ucharR_cons
+          (s_addr .[Tuchar ! 1] .[Tuchar ! 2])
+          100%Z [] with "Hs") as "Hs".
+        iDestruct "Hs" as "[#Hty3' [H3 Hempty2]]".
+        iEval (rewrite o_sub_sub) in "H3".
+        Arith.arith_simpl.
+        iExists (Vint 100%Z), (cQp.mk false 1%Qp).
+        iFrame "H3". iIntros "H3".
+        go.
+        iPoseProof (at_zero_elim s_addr with "H0_assert") as "H0".
+        iPoseProof (uchar_cells_object_bytesR_two s_addr 120%Z 120%Z
+          with "[$H0 $H1]") as "Hhead".
+        iPoseProof (at_uchar_offset_add_intro s_addr 2 1 3
+          (ucharR 1$m 100%Z) ltac:(lia) with "H3") as "H3".
+        iPoseProof (uchar_cells_object_bytesR_two (s_addr .[Tuchar ! 2])
+          35%Z 100%Z with "[$H2 $H3]") as "Htail".
+        iPoseProof ((object_bytesR_prefix_tail0 s_addr Tuchar
+          (cQp.mk false 1) 2 4 [120%Z; 120%Z] [35%Z; 100%Z]
+          ltac:(reflexivity) ltac:(reflexivity) ltac:(reflexivity))
+          with "[$Hhead $Htail]") as "Hs".
+        iPoseProof (object_bytesR_ucharR_arrayLR_anyR _ 4%N
+          [120%Z; 120%Z; 35%Z; 100%Z] ltac:(reflexivity) with "Hs")
+          as "Hs".
+        iFrame "Hs".
+        go.
+  Qed.
+
+  cpp.spec "test_memchr()" default.
+  Lemma test_memchr_ok : verify[module] "test_memchr()".
+  Proof using MOD _Σ thread_info Σ σ.
+    verify_spec; go.
+    iDestruct select (s_addr |-> arrayLR Tuchar 0 4
+      (fun v : Z => ucharR 1$m v) [97%Z; 98%Z; 99%Z; 97%Z]) as "Hs".
+    iPoseProof (object_bytesR_of_arrayLR s_addr Tuchar (cQp.mk false 1)
+      4 [97%Z; 98%Z; 99%Z; 97%Z] ltac:(reflexivity) with "Hs") as "Hs".
+    iExists Tuchar, (cQp.mk false 1), [97%Z; 98%Z; 99%Z; 97%Z].
+    iSplitL "Hs"; [iExact "Hs"|].
+    iSplit.
+      + done.
+      + iIntros "Hs".
+        rewrite (memchr_found_after_prefix (@nil Z) 97%Z [98%Z; 99%Z; 97%Z] 97%Z); [|solve_memchr_side..].
+        Arith.arith_simpl; go.
+    iExists Tuchar, (cQp.mk false 1), [97%Z; 98%Z; 99%Z; 97%Z].
+    iSplitL "Hs"; [iExact "Hs"|].
+    iSplit; [done|].
+    iIntros "Hs".
+    rewrite (memchr_found_after_prefix [97%Z; 98%Z] 99%Z [97%Z] 99%Z); [|solve_memchr_side..].
+    Arith.arith_simpl; go.
+    iExists Tuchar, (cQp.mk false 1), [97%Z; 98%Z; 99%Z; 97%Z].
+    iSplitL "Hs"; [iFrame|].
+    iSplit; [done|].
+    iIntros "Hs".
+    rewrite (memchr_missing_if_no_match [97%Z; 98%Z; 99%Z; 97%Z] 122%Z); [|solve_memchr_side..].
+    go.
+    iPoseProof (object_bytesR_prefix_tail0 s_addr Tuchar
+      (cQp.mk false 1) 0 4 [] [97%Z; 98%Z; 99%Z; 97%Z]
+      ltac:(reflexivity) ltac:(reflexivity) ltac:(reflexivity) with "Hs")
+      as "[Hempty Hs]".
+    iExists Tuchar, (cQp.mk false 1), [].
+    iSplitL "Hempty"; [iExact "Hempty"|].
+    iSplit; [done|].
+    iIntros "Hempty".
+    go.
+    iPoseProof ((object_bytesR_prefix_tail0 s_addr Tuchar
+      (cQp.mk false 1) 0 4 [] [97%Z; 98%Z; 99%Z; 97%Z]
+      ltac:(reflexivity) ltac:(reflexivity) ltac:(reflexivity))
+      with "[$Hempty $Hs]")
+      as "Hs".
+    iPoseProof (object_bytesR_prefix_tail0 s_addr Tuchar
+      (cQp.mk false 1) 1 4 [97%Z] [98%Z; 99%Z; 97%Z]
+      ltac:(reflexivity) ltac:(reflexivity) ltac:(reflexivity) with "Hs")
+      as "[Hhead Hs]".
+    iExists Tuchar, (cQp.mk false 1), [98%Z; 99%Z; 97%Z].
+    iSplitL "Hs"; [iExact "Hs"|].
+    iSplit; [done|].
+    iIntros "Hs".
+    rewrite (memchr_found_after_prefix [98%Z; 99%Z] 97%Z (@nil Z) 97%Z); [|solve_memchr_side..].
+    Arith.arith_simpl; go.
+    go.
+    iPoseProof ((object_bytesR_prefix_tail0 s_addr Tuchar
+      (cQp.mk false 1) 1 4 [97%Z] [98%Z; 99%Z; 97%Z]
+      ltac:(reflexivity) ltac:(reflexivity) ltac:(reflexivity))
+      with "[$Hhead $Hs]")
+      as "Hs".
+    iPoseProof (object_bytesR_ucharR_arrayLR_anyR _ 4%N
+      [97%Z; 98%Z; 99%Z; 97%Z]
+      ltac:(reflexivity) with "Hs") as "Hs".
+    iFrame "Hs".
+    go.
+    rewrite o_sub_sub in H.
+    simpl in H.
+    contradiction.
+  Qed.
+
+  cpp.spec "test_memchr_embedded_null()" default.
+  Lemma test_memchr_embedded_null_ok :
+    verify[module] "test_memchr_embedded_null()".
+  Proof using MOD _Σ thread_info Σ σ.
+    verify_spec; go.
+    iDestruct select (s_addr |-> arrayLR Tuchar 0 4
+      (fun v : Z => ucharR 1$m v) [97%Z; 0%Z; 98%Z; 0%Z]) as "Hs".
+    iPoseProof (object_bytesR_of_arrayLR s_addr Tuchar (cQp.mk false 1)
+      4 [97%Z; 0%Z; 98%Z; 0%Z] ltac:(reflexivity) with "Hs") as "Hs".
+    iExists Tuchar, (cQp.mk false 1), [97%Z; 0%Z; 98%Z; 0%Z].
+    iSplitL "Hs"; [iExact "Hs"|].
+    iSplit.
+    + done.
+    + iIntros "Hs".
+      rewrite (memchr_found_after_prefix [97%Z] 0%Z [98%Z; 0%Z] 0%Z); [|solve_memchr_side..].
+      Arith.arith_simpl; go.
+    iPoseProof (object_bytesR_prefix_tail0 s_addr Tuchar
+      (cQp.mk false 1) 2 4 [97%Z; 0%Z] [98%Z; 0%Z]
+      ltac:(reflexivity) ltac:(reflexivity) ltac:(reflexivity) with "Hs")
+      as "[Hhead Hs]".
+    iExists Tuchar, (cQp.mk false 1), [98%Z; 0%Z].
+    iSplitL "Hs"; [iExact "Hs"|].
+    iSplit; [done|].
+    iIntros "Hs".
+    rewrite (memchr_found_after_prefix [98%Z] 0%Z (@nil Z) 0%Z); [|solve_memchr_side..].
+    Arith.arith_simpl; go.
+    rewrite o_sub_sub.
+    Arith.arith_simpl.
+    go.
+    iPoseProof ((object_bytesR_prefix_tail0 s_addr Tuchar
+      (cQp.mk false 1) 2 4 [97%Z; 0%Z] [98%Z; 0%Z]
+      ltac:(reflexivity) ltac:(reflexivity) ltac:(reflexivity))
+      with "[$Hhead $Hs]")
+      as "Hs".
+    iExists Tuchar, (cQp.mk false 1), [97%Z; 0%Z; 98%Z; 0%Z].
+    iSplitL "Hs"; [iExact "Hs"|].
+    iSplit; [done|].
+    iIntros "Hs".
+    rewrite (memchr_found_after_prefix [97%Z; 0%Z] 98%Z [0%Z] 98%Z); [|solve_memchr_side..].
+    Arith.arith_simpl; go.
+    iPoseProof (object_bytesR_ucharR_arrayLR_anyR _ 4%N
+      [97%Z; 0%Z; 98%Z; 0%Z]
+      ltac:(reflexivity) with "Hs") as "Hs".
+    iFrame "Hs".
+    go.
+    rewrite o_sub_sub in H.
+    simpl in H.
+    contradiction.
+  Qed.
+
+  cpp.spec "test_memcpy()" default.
+  Lemma test_memcpy_ok : verify[module] "test_memcpy()".
+  Proof using MOD _Σ thread_info Σ σ.
+    verify_spec; go.
+    iDestruct select (src_addr |-> arrayLR Tuchar 0 4
+      (fun v : Z => ucharR 1$m v) [97%Z; 98%Z; 99%Z; 100%Z]) as "Hsrc".
+    iDestruct select (dst_addr |-> arrayLR Tuchar 0 4
+      (fun v : Z => ucharR 1$m v) [119%Z; 120%Z; 121%Z; 122%Z]) as "Hdst".
+
+    iPoseProof (object_bytesR_of_arrayLR src_addr Tuchar (cQp.mk false 1)
+      4 [97%Z; 98%Z; 99%Z; 100%Z] ltac:(reflexivity) with "Hsrc") as "Hsrc".
+    iPoseProof (object_bytesR_prefix_tail0 src_addr Tuchar
+      (cQp.mk false 1) 3 4 [97%Z; 98%Z; 99%Z] [100%Z]
+      ltac:(reflexivity) ltac:(reflexivity) ltac:(reflexivity) with "Hsrc")
+      as "[Hsrc_copy Hsrc_tail]".
+
+    iPoseProof (object_bytesR_of_arrayLR dst_addr Tuchar (cQp.mk false 1)
+      4 [119%Z; 120%Z; 121%Z; 122%Z] ltac:(reflexivity) with "Hdst") as "Hdst".
+    iPoseProof (object_bytesR_prefix_tail0 dst_addr Tuchar
+      (cQp.mk false 1) 3 4 [119%Z; 120%Z; 121%Z] [122%Z]
+      ltac:(reflexivity) ltac:(reflexivity) ltac:(reflexivity) with "Hdst")
+      as "[Hdst_copy Hdst_tail]".
+
+    iExists Tuchar, (cQp.mk false 1), [97%Z; 98%Z; 99%Z].
+    iExists Tuchar.
+    iSplitL "Hsrc_copy"; [iExact "Hsrc_copy"|].
+    iSplitL "Hdst_copy".
+    - iApply (object_bytesR_ucharR_object_bytes_anyR _ 3%N
+        [119%Z; 120%Z; 121%Z] ltac:(reflexivity) with "Hdst_copy").
+    - iSplit; [done|].
+      iIntros "[Hsrc_copy Hdst_copy]".
+      Arith.arith_simpl.
+      go.
+
+      iPoseProof ((object_bytesR_prefix_tail0 src_addr Tuchar
+        (cQp.mk false 1) 3 4 [97%Z; 98%Z; 99%Z] [100%Z]
+        ltac:(reflexivity) ltac:(reflexivity) ltac:(reflexivity))
+        with "[$Hsrc_copy $Hsrc_tail]") as "Hsrc".
+      iPoseProof ((object_bytesR_prefix_tail0 dst_addr Tuchar
+        (cQp.mk false 1) 3 4 [97%Z; 98%Z; 99%Z] [122%Z]
+        ltac:(reflexivity) ltac:(reflexivity) ltac:(reflexivity))
+        with "[$Hdst_copy $Hdst_tail]") as "Hdst".
+
+      iPoseProof (object_bytesR_ucharR_arrayR with "Hdst") as "Hdst".
+      rewrite (at_arrayR_ucharR_cons dst_addr 97%Z
+        [98%Z; 99%Z; 122%Z]).
+      iDestruct "Hdst" as "[#Hdst_ty0 [Hdst0 Hdst]]".
+      iPoseProof (at_zero_intro dst_addr with "Hdst0") as "Hdst0".
+      iExists (Vint 97%Z), (cQp.mk false 1%Qp).
+      iFrame "Hdst0". iIntros "Hdst0".
+      go.
+
+      iPoseProof (at_arrayR_ucharR_cons (dst_addr .[Tuchar ! 1])
+        98%Z [99%Z; 122%Z] with "Hdst") as "Hdst".
+      iDestruct "Hdst" as "[#Hdst_ty1 [Hdst1 Hdst]]".
+      iExists (Vint 98%Z), (cQp.mk false 1%Qp).
+      iFrame "Hdst1". iIntros "Hdst1".
+      go.
+
+      iPoseProof (at_arrayR_ucharR_cons (dst_addr .[Tuchar ! 1] .[Tuchar ! 1])
+        99%Z [122%Z] with "Hdst") as "Hdst".
+      iDestruct "Hdst" as "[#Hdst_ty2 [Hdst2 Hdst]]".
+      iEval (rewrite o_sub_sub) in "Hdst2".
+      iEval (rewrite o_sub_sub) in "Hdst".
+      Arith.arith_simpl.
+      iExists (Vint 99%Z), (cQp.mk false 1%Qp).
+      iFrame "Hdst2". iIntros "Hdst2".
+      go.
+
+      iPoseProof (at_arrayR_ucharR_cons
+        (dst_addr .[Tuchar ! 1] .[Tuchar ! 2])
+        122%Z [] with "Hdst") as "Hdst".
+      iDestruct "Hdst" as "[#Hdst_ty3 [Hdst3 Hdst]]".
+      iEval (rewrite o_sub_sub) in "Hdst".
+      Arith.arith_simpl.
+      iPoseProof (at_uchar_offset_add_elim dst_addr 1 2 3
+        (ucharR 1$m 122%Z) ltac:(lia) with "Hdst3") as "Hdst3".
+      iExists (Vint 122%Z), (cQp.mk false 1%Qp).
+      iFrame "Hdst3". iIntros "Hdst3".
+      go.
+
+      iPoseProof (object_bytesR_ucharR_arrayR with "Hsrc") as "Hsrc".
+      rewrite (at_arrayR_ucharR_cons src_addr 97%Z
+        [98%Z; 99%Z; 100%Z]).
+      iDestruct "Hsrc" as "[#Hsrc_ty0 [Hsrc0 Hsrc]]".
+      iPoseProof (at_zero_intro src_addr with "Hsrc0") as "Hsrc0".
+      iExists (Vint 97%Z), (cQp.mk false 1%Qp).
+      iFrame "Hsrc0". iIntros "Hsrc0".
+      go.
+
+      iPoseProof (at_arrayR_ucharR_cons (src_addr .[Tuchar ! 1])
+        98%Z [99%Z; 100%Z] with "Hsrc") as "Hsrc".
+      iDestruct "Hsrc" as "[#Hsrc_ty1 [Hsrc1 Hsrc]]".
+      iPoseProof (at_arrayR_ucharR_cons
+        (src_addr .[Tuchar ! 1] .[Tuchar ! 1])
+        99%Z [100%Z] with "Hsrc") as "Hsrc".
+      iDestruct "Hsrc" as "[#Hsrc_ty2 [Hsrc2 Hsrc]]".
+      iPoseProof (at_arrayR_ucharR_cons
+        (src_addr .[Tuchar ! 1] .[Tuchar ! 1] .[Tuchar ! 1])
+        100%Z [] with "Hsrc") as "Hsrc".
+      iDestruct "Hsrc" as "[#Hsrc_ty3 [Hsrc3 Hsrc]]".
+      iEval (rewrite o_sub_sub) in "Hsrc2".
+      iEval (rewrite o_sub_sub) in "Hsrc3".
+      iEval (rewrite o_sub_sub) in "Hsrc".
+      Arith.arith_simpl.
+      iPoseProof (at_uchar_offset_add_elim src_addr 1 2 3
+        (ucharR 1$m 100%Z) ltac:(lia) with "Hsrc3") as "Hsrc3".
+      iExists (Vint 100%Z), (cQp.mk false 1%Qp).
+      iFrame "Hsrc3". iIntros "Hsrc3".
+      go.
+
+      iPoseProof (at_zero_elim src_addr with "Hsrc0") as "Hsrc0".
+      iPoseProof (uchar_cells_object_bytesR_two src_addr 97%Z 98%Z
+        with "[$Hsrc0 $Hsrc1]") as "Hsrc_head".
+      iPoseProof (at_uchar_offset_add_intro src_addr 2 1 3
+        (ucharR 1$m 100%Z) ltac:(lia) with "Hsrc3") as "Hsrc3".
+      iPoseProof (uchar_cells_object_bytesR_two (src_addr .[Tuchar ! 2])
+        99%Z 100%Z with "[$Hsrc2 $Hsrc3]") as "Hsrc_tail2".
+      iPoseProof ((object_bytesR_prefix_tail0 src_addr Tuchar
+        (cQp.mk false 1) 2 4 [97%Z; 98%Z] [99%Z; 100%Z]
+        ltac:(reflexivity) ltac:(reflexivity) ltac:(reflexivity))
+        with "[$Hsrc_head $Hsrc_tail2]") as "Hsrc_full".
+
+      iPoseProof (at_zero_elim dst_addr with "Hdst0") as "Hdst0".
+      iPoseProof (uchar_cells_object_bytesR_two dst_addr 97%Z 98%Z
+        with "[$Hdst0 $Hdst1]") as "Hdst_head".
+      iPoseProof (at_uchar_offset_add_intro dst_addr 2 1 3
+        (ucharR 1$m 122%Z) ltac:(lia) with "Hdst3") as "Hdst3".
+      iPoseProof (uchar_cells_object_bytesR_two (dst_addr .[Tuchar ! 2])
+        99%Z 122%Z with "[$Hdst2 $Hdst3]") as "Hdst_tail2".
+      iPoseProof ((object_bytesR_prefix_tail0 dst_addr Tuchar
+        (cQp.mk false 1) 2 4 [97%Z; 98%Z] [99%Z; 122%Z]
+        ltac:(reflexivity) ltac:(reflexivity) ltac:(reflexivity))
+        with "[$Hdst_head $Hdst_tail2]") as "Hdst_full".
+
+      iPoseProof (object_bytesR_prefix_tail0 src_addr Tuchar
+        (cQp.mk false 1) 2 4 [97%Z; 98%Z] [99%Z; 100%Z]
+        ltac:(reflexivity) ltac:(reflexivity) ltac:(reflexivity) with "Hsrc_full")
+        as "[Hsrc_prefix Hsrc_suffix]".
+      iPoseProof (object_bytesR_prefix_tail0 (src_addr .[Tuchar ! 2]) Tuchar
+        (cQp.mk false 1) 0 2 [] [99%Z; 100%Z]
+        ltac:(reflexivity) ltac:(reflexivity) ltac:(reflexivity)
+        with "Hsrc_suffix") as "[Hsrc_empty Hsrc_suffix]".
+
+      iPoseProof (object_bytesR_prefix_tail0 dst_addr Tuchar
+        (cQp.mk false 1) 1 4 [97%Z] [98%Z; 99%Z; 122%Z]
+        ltac:(reflexivity) ltac:(reflexivity) ltac:(reflexivity) with "Hdst_full")
+        as "[Hdst_head1 Hdst_suffix]".
+      iPoseProof (object_bytesR_prefix_tail0 (dst_addr .[Tuchar ! 1]) Tuchar
+        (cQp.mk false 1) 0 3 [] [98%Z; 99%Z; 122%Z]
+        ltac:(reflexivity) ltac:(reflexivity) ltac:(reflexivity)
+        with "Hdst_suffix") as "[Hdst_empty Hdst_suffix]".
+
+      iExists Tuchar, (cQp.mk false 1), [].
+      iExists Tuchar.
+      iSplitL "Hsrc_empty"; [iExact "Hsrc_empty"|].
+      iSplitL "Hdst_empty".
+      + iApply (object_bytesR_ucharR_object_bytes_anyR _ 0%N
+          [] ltac:(reflexivity) with "Hdst_empty").
+      + iSplit; [done|].
+        iIntros "[Hsrc_empty Hdst_empty]".
+        Arith.arith_simpl.
+        go.
+
+        iPoseProof ((object_bytesR_prefix_tail0 (src_addr .[Tuchar ! 2]) Tuchar
+          (cQp.mk false 1) 0 2 [] [99%Z; 100%Z]
+          ltac:(reflexivity) ltac:(reflexivity) ltac:(reflexivity))
+          with "[$Hsrc_empty $Hsrc_suffix]") as "Hsrc_suffix".
+        iPoseProof ((object_bytesR_prefix_tail0 src_addr Tuchar
+          (cQp.mk false 1) 2 4 [97%Z; 98%Z] [99%Z; 100%Z]
+          ltac:(reflexivity) ltac:(reflexivity) ltac:(reflexivity))
+          with "[$Hsrc_prefix $Hsrc_suffix]") as "Hsrc_full".
+
+        iPoseProof ((object_bytesR_prefix_tail0 (dst_addr .[Tuchar ! 1]) Tuchar
+          (cQp.mk false 1) 0 3 [] [98%Z; 99%Z; 122%Z]
+          ltac:(reflexivity) ltac:(reflexivity) ltac:(reflexivity))
+          with "[$Hdst_empty $Hdst_suffix]") as "Hdst_suffix".
+        iPoseProof ((object_bytesR_prefix_tail0 dst_addr Tuchar
+          (cQp.mk false 1) 1 4 [97%Z] [98%Z; 99%Z; 122%Z]
+          ltac:(reflexivity) ltac:(reflexivity) ltac:(reflexivity))
+          with "[$Hdst_head1 $Hdst_suffix]") as "Hdst_full".
+
+        iPoseProof (object_bytesR_ucharR_arrayR with "Hdst_full") as "Hdst_arr".
+        rewrite (at_arrayR_ucharR_cons dst_addr 97%Z
+          [98%Z; 99%Z; 122%Z]).
+        iDestruct "Hdst_arr" as "[#Hdst_ty4 [Hdst0 Hdst_arr]]".
+        iPoseProof (at_zero_intro dst_addr with "Hdst0") as "Hdst0".
+        iExists (Vint 97%Z), (cQp.mk false 1%Qp).
+        iFrame "Hdst0". iIntros "Hdst0".
+        go.
+
+        iPoseProof (at_arrayR_ucharR_cons (dst_addr .[Tuchar ! 1])
+          98%Z [99%Z; 122%Z] with "Hdst_arr") as "Hdst_arr".
+        iDestruct "Hdst_arr" as "[#Hdst_ty5 [Hdst1 Hdst_arr]]".
+        iExists (Vint 98%Z), (cQp.mk false 1%Qp).
+        iFrame "Hdst1". iIntros "Hdst1".
+        go.
+
+        iPoseProof (object_bytesR_ucharR_arrayLR_anyR _ 4%N
+          [97%Z; 98%Z; 99%Z; 100%Z] ltac:(reflexivity) with "Hsrc_full") as "Hsrc_any".
+        iPoseProof (at_zero_elim dst_addr with "Hdst0") as "Hdst0".
+        iPoseProof (uchar_cells_object_bytesR_two dst_addr 97%Z 98%Z
+          with "[$Hdst0 $Hdst1]") as "Hdst_head".
+        iEval (rewrite (at_arrayR_ucharR_cons
+          (dst_addr .[Tuchar ! 1] .[Tuchar ! 1]) 99%Z [122%Z]))
+          in "Hdst_arr".
+        iDestruct "Hdst_arr" as "[#Hdst_ty6 [Hdst2 Hdst_arr]]".
+        iPoseProof (at_arrayR_ucharR_cons
+          (dst_addr .[Tuchar ! 1] .[Tuchar ! 1] .[Tuchar ! 1])
+          122%Z [] with "Hdst_arr") as "Hdst_arr".
+        iDestruct "Hdst_arr" as "[#Hdst_ty7 [Hdst3 Hdst_arr]]".
+        iEval (rewrite o_sub_sub) in "Hdst2".
+        iEval (rewrite o_sub_sub) in "Hdst3".
+        iEval (rewrite o_sub_sub) in "Hdst3".
+        iPoseProof (at_uchar_offset_add_intro dst_addr 2 1 3
+          (ucharR 1$m 122%Z) ltac:(lia) with "Hdst3") as "Hdst3".
+        iPoseProof (uchar_cells_object_bytesR_two (dst_addr .[Tuchar ! 2])
+          99%Z 122%Z with "[$Hdst2 $Hdst3]") as "Hdst_tail2".
+        iPoseProof ((object_bytesR_prefix_tail0 dst_addr Tuchar
+          (cQp.mk false 1) 2 4 [97%Z; 98%Z] [99%Z; 122%Z]
+          ltac:(reflexivity) ltac:(reflexivity) ltac:(reflexivity))
+          with "[$Hdst_head $Hdst_tail2]") as "Hdst_full".
+        iPoseProof (object_bytesR_ucharR_arrayLR_anyR _ 4%N
+          [97%Z; 98%Z; 99%Z; 122%Z] ltac:(reflexivity) with "Hdst_full") as "Hdst_any".
+        iFrame "Hsrc_any Hdst_any".
+        go.
+  Qed.
+
+  cpp.spec "test_memmove()" default.
+  Lemma test_memmove_ok : verify[module] "test_memmove()".
+  Proof using MOD _Σ thread_info Σ σ.
+    verify_spec; go.
+    iDestruct select (src_addr |-> arrayLR Tuchar 0 4
+      (fun v : Z => ucharR 1$m v) [97%Z; 98%Z; 99%Z; 100%Z]) as "Hsrc".
+    iDestruct select (dst_addr |-> arrayLR Tuchar 0 4
+      (fun v : Z => ucharR 1$m v) [119%Z; 120%Z; 121%Z; 122%Z]) as "Hdst".
+
+    iPoseProof (object_bytesR_of_arrayLR src_addr Tuchar (cQp.mk false 1)
+      4 [97%Z; 98%Z; 99%Z; 100%Z] ltac:(reflexivity) with "Hsrc") as "Hsrc".
+    iPoseProof (object_bytesR_of_arrayLR dst_addr Tuchar (cQp.mk false 1)
+      4 [119%Z; 120%Z; 121%Z; 122%Z] ltac:(reflexivity) with "Hdst") as "Hdst".
+
+    iExists Tuchar, (cQp.mk false 1), [97%Z; 98%Z; 99%Z; 100%Z].
+    iExists Tuchar.
+    iSplitL "Hsrc"; [iExact "Hsrc"|].
+    iSplitL "Hdst".
+    - iApply (object_bytesR_ucharR_object_bytes_anyR _ 4%N
+        [119%Z; 120%Z; 121%Z; 122%Z] ltac:(reflexivity) with "Hdst").
+    - iSplit; [done|].
+      iIntros "[Hsrc Hdst]".
+      Arith.arith_simpl.
+      go.
+
+      iPoseProof (object_bytesR_ucharR_arrayR with "Hdst") as "Hdst_arr".
+      rewrite (at_arrayR_ucharR_cons dst_addr 97%Z
+        [98%Z; 99%Z; 100%Z]).
+      iDestruct "Hdst_arr" as "[#Hdst_ty0 [Hdst0 Hdst_arr]]".
+      iPoseProof (at_zero_intro dst_addr with "Hdst0") as "Hdst0".
+      iExists (Vint 97%Z), (cQp.mk false 1%Qp).
+      iFrame "Hdst0". iIntros "Hdst0".
+      go.
+
+      iPoseProof (at_arrayR_ucharR_cons (dst_addr .[Tuchar ! 1])
+        98%Z [99%Z; 100%Z] with "Hdst_arr") as "Hdst_arr".
+      iDestruct "Hdst_arr" as "[#Hdst_ty1 [Hdst1 Hdst_arr]]".
+      iExists (Vint 98%Z), (cQp.mk false 1%Qp).
+      iFrame "Hdst1". iIntros "Hdst1".
+      go.
+
+      iPoseProof (at_arrayR_ucharR_cons
+        (dst_addr .[Tuchar ! 1] .[Tuchar ! 1])
+        99%Z [100%Z] with "Hdst_arr") as "Hdst_arr".
+      iDestruct "Hdst_arr" as "[#Hdst_ty2 [Hdst2 Hdst_arr]]".
+      iEval (rewrite o_sub_sub) in "Hdst2".
+      iEval (rewrite o_sub_sub) in "Hdst_arr".
+      Arith.arith_simpl.
+      iExists (Vint 99%Z), (cQp.mk false 1%Qp).
+      iFrame "Hdst2". iIntros "Hdst2".
+      go.
+
+      iPoseProof (at_arrayR_ucharR_cons
+        (dst_addr .[Tuchar ! 1] .[Tuchar ! 2])
+        100%Z [] with "Hdst_arr") as "Hdst_arr".
+      iDestruct "Hdst_arr" as "[#Hdst_ty3 [Hdst3 Hdst_arr]]".
+      iEval (rewrite o_sub_sub) in "Hdst_arr".
+      Arith.arith_simpl.
+      iPoseProof (at_uchar_offset_add_elim dst_addr 1 2 3
+        (ucharR 1$m 100%Z) ltac:(lia) with "Hdst3") as "Hdst3".
+      iExists (Vint 100%Z), (cQp.mk false 1%Qp).
+      iFrame "Hdst3". iIntros "Hdst3".
+      go.
+
+      iPoseProof (at_zero_elim dst_addr with "Hdst0") as "Hdst0".
+      iPoseProof (uchar_cells_object_bytesR_two dst_addr 97%Z 98%Z
+        with "[$Hdst0 $Hdst1]") as "Hdst_head".
+      iPoseProof (at_uchar_offset_add_intro dst_addr 2 1 3
+        (ucharR 1$m 100%Z) ltac:(lia) with "Hdst3") as "Hdst3".
+      iPoseProof (uchar_cells_object_bytesR_two (dst_addr .[Tuchar ! 2])
+        99%Z 100%Z with "[$Hdst2 $Hdst3]") as "Hdst_tail2".
+      iPoseProof ((object_bytesR_prefix_tail0 dst_addr Tuchar
+        (cQp.mk false 1) 2 4 [97%Z; 98%Z] [99%Z; 100%Z]
+        ltac:(reflexivity) ltac:(reflexivity) ltac:(reflexivity))
+        with "[$Hdst_head $Hdst_tail2]") as "Hdst_full".
+
+      iPoseProof (object_bytesR_prefix_tail0 src_addr Tuchar
+        (cQp.mk false 1) 1 4 [97%Z] [98%Z; 99%Z; 100%Z]
+        ltac:(reflexivity) ltac:(reflexivity) ltac:(reflexivity) with "Hsrc")
+        as "[Hsrc_head1 Hsrc_suffix]".
+      iPoseProof (object_bytesR_prefix_tail0 (src_addr .[Tuchar ! 1]) Tuchar
+        (cQp.mk false 1) 0 3 [] [98%Z; 99%Z; 100%Z]
+        ltac:(reflexivity) ltac:(reflexivity) ltac:(reflexivity)
+        with "Hsrc_suffix") as "[Hsrc_empty Hsrc_suffix]".
+
+      iPoseProof (object_bytesR_prefix_tail0 dst_addr Tuchar
+        (cQp.mk false 1) 1 4 [97%Z] [98%Z; 99%Z; 100%Z]
+        ltac:(reflexivity) ltac:(reflexivity) ltac:(reflexivity) with "Hdst_full")
+        as "[Hdst_head1 Hdst_suffix]".
+      iPoseProof (object_bytesR_prefix_tail0 (dst_addr .[Tuchar ! 1]) Tuchar
+        (cQp.mk false 1) 0 3 [] [98%Z; 99%Z; 100%Z]
+        ltac:(reflexivity) ltac:(reflexivity) ltac:(reflexivity)
+        with "Hdst_suffix") as "[Hdst_empty Hdst_suffix]".
+
+      iExists Tuchar, (cQp.mk false 1), [].
+      iExists Tuchar.
+      iSplitL "Hsrc_empty"; [iExact "Hsrc_empty"|].
+      iSplitL "Hdst_empty".
+      + iApply (object_bytesR_ucharR_object_bytes_anyR _ 0%N
+          [] ltac:(reflexivity) with "Hdst_empty").
+      + iSplit; [done|].
+        iIntros "[Hsrc_empty Hdst_empty]".
+        Arith.arith_simpl.
+        go.
+
+        iPoseProof ((object_bytesR_prefix_tail0 (src_addr .[Tuchar ! 1]) Tuchar
+          (cQp.mk false 1) 0 3 [] [98%Z; 99%Z; 100%Z]
+          ltac:(reflexivity) ltac:(reflexivity) ltac:(reflexivity))
+          with "[$Hsrc_empty $Hsrc_suffix]") as "Hsrc_suffix".
+        iPoseProof ((object_bytesR_prefix_tail0 src_addr Tuchar
+          (cQp.mk false 1) 1 4 [97%Z] [98%Z; 99%Z; 100%Z]
+          ltac:(reflexivity) ltac:(reflexivity) ltac:(reflexivity))
+          with "[$Hsrc_head1 $Hsrc_suffix]") as "Hsrc_full".
+
+        iPoseProof ((object_bytesR_prefix_tail0 (dst_addr .[Tuchar ! 1]) Tuchar
+          (cQp.mk false 1) 0 3 [] [98%Z; 99%Z; 100%Z]
+          ltac:(reflexivity) ltac:(reflexivity) ltac:(reflexivity))
+          with "[$Hdst_empty $Hdst_suffix]") as "Hdst_suffix".
+        iPoseProof ((object_bytesR_prefix_tail0 dst_addr Tuchar
+          (cQp.mk false 1) 1 4 [97%Z] [98%Z; 99%Z; 100%Z]
+          ltac:(reflexivity) ltac:(reflexivity) ltac:(reflexivity))
+          with "[$Hdst_head1 $Hdst_suffix]") as "Hdst_full".
+
+        iPoseProof (object_bytesR_ucharR_arrayR with "Hdst_full") as "Hdst_arr2".
+        rewrite (at_arrayR_ucharR_cons dst_addr 97%Z
+          [98%Z; 99%Z; 100%Z]).
+        iDestruct "Hdst_arr2" as "[#Hdst_ty4 [Hdst0 Hdst_arr2]]".
+        iPoseProof (at_zero_intro dst_addr with "Hdst0") as "Hdst0".
+        iPoseProof (at_arrayR_ucharR_cons (dst_addr .[Tuchar ! 1])
+          98%Z [99%Z; 100%Z] with "Hdst_arr2") as "Hdst_arr2".
+        iDestruct "Hdst_arr2" as "[#Hdst_ty5 [Hdst1 Hdst_arr2]]".
+        iExists (Vint 98%Z), (cQp.mk false 1%Qp).
+        iFrame "Hdst1". iIntros "Hdst1".
+        go.
+
+        iPoseProof (object_bytesR_ucharR_arrayLR_anyR _ 4%N
+          [97%Z; 98%Z; 99%Z; 100%Z] ltac:(reflexivity) with "Hsrc_full")
+          as "Hsrc_any".
+        iPoseProof (at_zero_elim dst_addr with "Hdst0") as "Hdst0".
+        iPoseProof (uchar_cells_object_bytesR_two dst_addr 97%Z 98%Z
+          with "[$Hdst0 $Hdst1]") as "Hdst_head".
+        iEval (rewrite (at_arrayR_ucharR_cons
+          (dst_addr .[Tuchar ! 1] .[Tuchar ! 1]) 99%Z [100%Z]))
+          in "Hdst_arr2".
+        iDestruct "Hdst_arr2" as "[#Hdst_ty6 [Hdst2 Hdst_arr3]]".
+        iPoseProof (at_arrayR_ucharR_cons
+          (dst_addr .[Tuchar ! 1] .[Tuchar ! 1] .[Tuchar ! 1])
+          100%Z [] with "Hdst_arr3") as "Hdst_arr3".
+        iDestruct "Hdst_arr3" as "[#Hdst_ty7 [Hdst3 Hdst_arr3]]".
+        iEval (rewrite o_sub_sub) in "Hdst2".
+        iEval (rewrite o_sub_sub) in "Hdst3".
+        iEval (rewrite o_sub_sub) in "Hdst3".
+        iPoseProof (at_uchar_offset_add_intro dst_addr 2 1 3
+          (ucharR 1$m 100%Z) ltac:(lia) with "Hdst3") as "Hdst3".
+        iPoseProof (uchar_cells_object_bytesR_two (dst_addr .[Tuchar ! 2])
+          99%Z 100%Z with "[$Hdst2 $Hdst3]") as "Hdst_tail2".
+        iPoseProof ((object_bytesR_prefix_tail0 dst_addr Tuchar
+          (cQp.mk false 1) 2 4 [97%Z; 98%Z] [99%Z; 100%Z]
+          ltac:(reflexivity) ltac:(reflexivity) ltac:(reflexivity))
+          with "[$Hdst_head $Hdst_tail2]") as "Hdst_full".
+        iPoseProof (object_bytesR_ucharR_arrayLR_anyR _ 4%N
+          [97%Z; 98%Z; 99%Z; 100%Z] ltac:(reflexivity) with "Hdst_full")
+          as "Hdst_any".
+        iFrame "Hsrc_any Hdst_any".
+        go.
+  Qed.
+
+  cpp.spec "test_memcmp()" default.
+  Lemma test_memcmp_ok : verify[module] "test_memcmp()".
+  Proof using MOD _Σ thread_info Σ σ.
+    verify_spec; go.
+    iDestruct select (abc_addr |-> arrayLR Tuchar 0 3
+      (fun v : Z => ucharR 1$m v) [97%Z; 98%Z; 99%Z]) as "Habc".
+    iDestruct select (abd_addr |-> arrayLR Tuchar 0 3
+      (fun v : Z => ucharR 1$m v) [97%Z; 98%Z; 100%Z]) as "Habd".
+    iDestruct select (ab_addr |-> arrayLR Tuchar 0 2
+      (fun v : Z => ucharR 1$m v) [97%Z; 98%Z]) as "Hab".
+
+    iPoseProof (object_bytesR_of_arrayLR abc_addr Tuchar (cQp.mk false 1)
+      3 [97%Z; 98%Z; 99%Z] ltac:(reflexivity) with "Habc") as "Habc".
+    iPoseProof (object_bytesR_half_split with "Habc") as
+      "[Habc_left Habc_right]".
+    iExists Tuchar, (cQp.mk false (1/2)), [97%Z; 98%Z; 99%Z].
+    iExists Tuchar, (cQp.mk false (1/2)), [97%Z; 98%Z; 99%Z].
+    iSplitL "Habc_left"; [iExact "Habc_left"|].
+    iSplitL "Habc_right"; [iExact "Habc_right"|].
+    iSplit; [done|].
+    iSplit; [done|].
+    iIntros "[Habc_left Habc_right]".
+    Arith.arith_simpl.
+    go.
+    iPoseProof ((object_bytesR_half_split abc_addr Tuchar
+      [97%Z; 98%Z; 99%Z]) with "[$Habc_left $Habc_right]") as "Habc".
+
+    iPoseProof (object_bytesR_of_arrayLR abd_addr Tuchar (cQp.mk false 1)
+      3 [97%Z; 98%Z; 100%Z] ltac:(reflexivity) with "Habd") as "Habd".
+    iExists Tuchar, (cQp.mk false 1), [97%Z; 98%Z; 99%Z].
+    iExists Tuchar, (cQp.mk false 1), [97%Z; 98%Z; 100%Z].
+    iSplitL "Habc"; [iExact "Habc"|].
+    iSplitL "Habd"; [iExact "Habd"|].
+    iSplit; [done|].
+    iSplit; [done|].
+    iIntros "[Habc Habd]".
+    Arith.arith_simpl.
+    go.
+
+    iExists Tuchar, (cQp.mk false 1), [97%Z; 98%Z; 100%Z].
+    iExists Tuchar, (cQp.mk false 1), [97%Z; 98%Z; 99%Z].
+    iSplitL "Habd"; [iExact "Habd"|].
+    iSplitL "Habc"; [iExact "Habc"|].
+    iSplit; [done|].
+    iSplit; [done|].
+    iIntros "[Habd Habc]".
+    Arith.arith_simpl.
+    go.
+
+    iPoseProof (object_bytesR_prefix_tail0 abc_addr Tuchar
+      (cQp.mk false 1) 2 3 [97%Z; 98%Z] [99%Z]
+      ltac:(reflexivity) ltac:(reflexivity) ltac:(reflexivity) with "Habc")
+      as "[Habc_prefix Habc_tail]".
+    iPoseProof (object_bytesR_prefix_tail0 abd_addr Tuchar
+      (cQp.mk false 1) 2 3 [97%Z; 98%Z] [100%Z]
+      ltac:(reflexivity) ltac:(reflexivity) ltac:(reflexivity) with "Habd")
+      as "[Habd_prefix Habd_tail]".
+    iExists Tuchar, (cQp.mk false 1), [97%Z; 98%Z].
+    iExists Tuchar, (cQp.mk false 1), [97%Z; 98%Z].
+    iSplitL "Habc_prefix"; [iExact "Habc_prefix"|].
+    iSplitL "Habd_prefix"; [iExact "Habd_prefix"|].
+    iSplit; [done|].
+    iSplit; [done|].
+    iIntros "[Habc_prefix Habd_prefix]".
+    Arith.arith_simpl.
+    go.
+    iPoseProof ((object_bytesR_prefix_tail0 abc_addr Tuchar
+      (cQp.mk false 1) 2 3 [97%Z; 98%Z] [99%Z]
+      ltac:(reflexivity) ltac:(reflexivity) ltac:(reflexivity))
+      with "[$Habc_prefix $Habc_tail]") as "Habc".
+    iPoseProof ((object_bytesR_prefix_tail0 abd_addr Tuchar
+      (cQp.mk false 1) 2 3 [97%Z; 98%Z] [100%Z]
+      ltac:(reflexivity) ltac:(reflexivity) ltac:(reflexivity))
+      with "[$Habd_prefix $Habd_tail]") as "Habd".
+
+    iPoseProof (object_bytesR_prefix_tail0 abc_addr Tuchar
+      (cQp.mk false 1) 0 3 [] [97%Z; 98%Z; 99%Z]
+      ltac:(reflexivity) ltac:(reflexivity) ltac:(reflexivity) with "Habc")
+      as "[Habc_empty Habc]".
+    iPoseProof (object_bytesR_of_arrayLR ab_addr Tuchar (cQp.mk false 1)
+      2 [97%Z; 98%Z] ltac:(reflexivity) with "Hab") as "Hab".
+    iPoseProof (object_bytesR_prefix_tail0 ab_addr Tuchar
+      (cQp.mk false 1) 0 2 [] [97%Z; 98%Z]
+      ltac:(reflexivity) ltac:(reflexivity) ltac:(reflexivity) with "Hab")
+      as "[Hab_empty Hab]".
+    iExists Tuchar, (cQp.mk false 1), [].
+    iExists Tuchar, (cQp.mk false 1), [].
+    iSplitL "Habc_empty"; [iExact "Habc_empty"|].
+    iSplitL "Hab_empty"; [iExact "Hab_empty"|].
+    iSplit; [done|].
+    iSplit; [done|].
+    iIntros "[Habc_empty Hab_empty]".
+    Arith.arith_simpl.
+    go.
+    iPoseProof ((object_bytesR_prefix_tail0 abc_addr Tuchar
+      (cQp.mk false 1) 0 3 [] [97%Z; 98%Z; 99%Z]
+      ltac:(reflexivity) ltac:(reflexivity) ltac:(reflexivity))
+      with "[$Habc_empty $Habc]") as "Habc".
+    iPoseProof ((object_bytesR_prefix_tail0 ab_addr Tuchar
+      (cQp.mk false 1) 0 2 [] [97%Z; 98%Z]
+      ltac:(reflexivity) ltac:(reflexivity) ltac:(reflexivity))
+      with "[$Hab_empty $Hab]") as "Hab".
+
+    iPoseProof (object_bytesR_ucharR_arrayLR_anyR _ 3%N
+      [97%Z; 98%Z; 99%Z] ltac:(reflexivity) with "Habc") as "Habc".
+    iPoseProof (object_bytesR_ucharR_arrayLR_anyR _ 3%N
+      [97%Z; 98%Z; 100%Z] ltac:(reflexivity) with "Habd") as "Habd".
+    iPoseProof (object_bytesR_ucharR_arrayLR_anyR _ 2%N
+      [97%Z; 98%Z] ltac:(reflexivity) with "Hab") as "Hab".
+    iFrame "Habc Habd Hab".
+    go.
+  Qed.
+
+  cpp.spec "test_memcmp_embedded_null()" default.
+
+  cpp.spec "test_memset_embedded_null()" default.
+
+  cpp.spec "test_memcpy_embedded_null()" default.
+
+  cpp.spec "test_memmove_overlap()" default.
+
+  cpp.spec "test_memmove_embedded_null()" default.
+
+  cpp.spec "test_cstring_slice4()" default.
 End with_cpp.
